Core/Algorithm/KindSound.lean
@@ -1,0 +1,56 @@
+import Core.Algorithm.Kind
+import Core.Ty
+import Core.Typing
+
+theorem wf_kind_sound :
+  wf_kind K == .some u -> Sorting K □ := by
+intro h
+induction K using wf_kind.induct
+all_goals (unfold wf_kind at h; simp at h)
+constructor
+constructor
+case _ ih1 ih2 =>
+rw[Option.bind_eq_some_iff] at h; rcases h with ⟨u1, h1, h⟩
+rw[Option.bind_eq_some_iff] at h; rcases h with ⟨u2, h2, h⟩
+cases h; cases u1; cases u2; cases u
+constructor
+replace h1 := beq_of_eq h1; apply ih1 h1
+replace h2 := beq_of_eq h2; apply ih2 h2
+
+theorem base_kind_some {k : Kind}:
+  k.base_kind = some b ->
+  k = .base b := by
+intro h
+induction k <;> simp at *
+case _ a =>
+  cases a
+  · unfold Kind.base_kind at h; simp at *; assumption
+  · unfold Kind.base_kind at h; simp at *; assumption
+case _ => unfold Kind.base_kind at h; simp at h
+
+
+theorem infer_kind_sound :
+  infer_kind G Δ τ = some k -> ⊢ G -> Kinding G Δ τ k := by
+intro h wf
+induction Δ, τ using infer_kind.induct generalizing k <;> simp at *
+all_goals( try
+  rw[Option.bind_eq_some_iff] at h; rcases h with ⟨_, _ , h⟩
+  rw[Option.bind_eq_some_iff] at h; rcases h with ⟨_, h, e3⟩
+  cases e3; constructor; assumption)
+case _ ih1 ih2 =>
+  rw[Option.bind_eq_some_iff] at h; rcases h with ⟨_, h1, h⟩
+  rw[Option.bind_eq_some_iff] at h; rcases h with ⟨_, h2, h⟩
+  rw[Option.bind_eq_some_iff] at h; rcases h with ⟨_, h3, h⟩
+  rw[Option.bind_eq_some_iff] at h; rcases h with ⟨_, h4, h⟩
+  rw[Option.bind_eq_some_iff] at h; rcases h with ⟨_, h5, h⟩
+  rw[Option.bind_eq_some_iff] at h; rcases h with ⟨_, h6, h⟩
+  simp at h; cases h.1; cases h.2; clear h
+  replace ih1 := ih1 h1
+  replace ih2 := ih2 h4
+  replace h3 := base_kind_some h3
+  replace h5 := base_kind_some h5
+  cases h3; cases h5
+  constructor; assumption; assumption
+sorry
+sorry
+sorry
